Coq/Simplicity/StaticAnalysis.v
@@ -1,0 +1,187 @@
+Require Import PeanoNat.
+Require Import Util.List.
+Require Import Util.Option.
+
+Require Import Simplicity.Alg.
+Require Import Simplicity.Core.
+Require Import Simplicity.BitMachine.
+Require Import Simplicity.Translate.
+Require Import Simplicity.Ty.
+
+Module StateShape.
+(* In this section we prove that executing Simplicity programs on the Bit
+ * Machine starting from *any* state, preserves the shape of the state (if it
+ * doesn't crash).
+ *)
+
+Definition spec {A B : Ty} (t : Term A B)  :=
+  forall x y, runMachine (@Core.eval _ _ t Naive.translate) x = Some y ->
+              stateShape x = stateShape y.
+
+Lemma iden_spec {A : Ty} : spec (@iden A).
+Proof.
+intros x y; simpl.
+unfold copy, runMachine.
+destruct (Copy_chk _ _) as [[[l st] [_ ->]] |];[simpl|discriminate].
+intros Hxy; inversion_clear Hxy.
+do 2 rewrite fillContextShape_correct.
+unfold localStateShape; simpl.
+rewrite fullWriteFrame_size.
+reflexivity.
+Qed.
+
+Lemma unit_spec {A : Ty} : spec (@unit A).
+Proof.
+intros x y Hxy.
+inversion_clear Hxy.
+reflexivity.
+Qed.
+
+Lemma comp_spec {A B C : Ty} (s : Term A B) (t : Term B C) :
+ spec s -> spec t -> spec (comp s t) .
+Proof.
+intros Hs Ht x z; cbn.
+repeat rewrite runMachine_seq; cbn.
+set (x1 := Build_State _ _ _ _); specialize (Hs x1).
+destruct (runMachine _ x1) as [y0|];[cbn|discriminate].
+specialize (Hs _ (eq_refl _)).
+unfold moveFrame, runMachine at 3.
+destruct (MoveFrame_chk _) as [[[l0 st0] ->] |];[cbn|discriminate].
+set (y1 := Build_State _ _ _ _); specialize (Ht y1).
+destruct (runMachine _ y1) as [z0|];[cbn|discriminate].
+specialize (Ht _ (eq_refl _)).
+unfold dropFrame, runMachine.
+destruct (DropFrame_chk _) as [[[l1 st1] ->] |];[cbn|discriminate].
+intros Hz; inversion Hz as [Hz0]; rewrite <- Hz0; clear z Hz Hz0.
+destruct x as [irf arf awf iwf];
+unfold stateShape in *; cbn in *.
+inversion Hs as [[Hs0 Hs1 Hs2 Hs3 Hs4]].
+rewrite Hs0, Hs1, Hs3, Hs4.
+clear x1 Hs Hs0 Hs1 Hs2 Hs3 Hs4.
+inversion_clear Ht.
+reflexivity.
+Qed.
+
+Lemma injl_spec {A B C : Ty} (t : Term A B) :
+ spec t -> spec (@injl A B C t).
+Proof.
+intros ht x y; cbn.
+repeat rewrite runMachine_seq.
+unfold write, runMachine at 3.
+destruct (Write_chk _) as [[ctx ->] |];[cbn|discriminate].
+set (x0 := fillContext _ _).
+replace (stateShape _) with (stateShape x0).
+ unfold skip, runMachine at 2.
+ destruct (Skip_chk _ _) as [[ctx0 ->] |];[cbn|discriminate].
+ intros Hx1.
+ rewrite <- (ht _ _ Hx1); clear y ht Hx1.
+ do 2 rewrite fillContextShape_correct.
+ unfold localStateShape; simpl.
+ rewrite fullWriteFrame_size, repeat_length.
+ reflexivity.
+unfold x0; do 2 rewrite fillContextShape_correct.
+unfold localStateShape; simpl.
+rewrite fullWriteFrame_size.
+reflexivity.
+Qed.
+
+Lemma injr_spec {A B C : Ty} (t : Term A C) :
+ spec t -> spec (@injr A B C t).
+Proof.
+intros ht x y; cbn.
+repeat rewrite runMachine_seq.
+unfold write, runMachine at 3.
+destruct (Write_chk _) as [[ctx ->] |];[cbn|discriminate].
+set (x0 := fillContext _ _).
+replace (stateShape _) with (stateShape x0).
+ unfold skip, runMachine at 2.
+ destruct (Skip_chk _ _) as [[ctx0 ->] |];[cbn|discriminate].
+ intros Hx1.
+ rewrite <- (ht _ _ Hx1); clear y ht Hx1.
+ do 2 rewrite fillContextShape_correct.
+ unfold localStateShape; simpl.
+ rewrite fullWriteFrame_size, repeat_length.
+ reflexivity.
+unfold x0; do 2 rewrite fillContextShape_correct.
+unfold localStateShape; simpl.
+rewrite fullWriteFrame_size.
+reflexivity.
+Qed.
+
+Lemma bump_spec {A B : Ty} (t : Term A B) n (Ht : spec t) x y :
+ runMachine (bump n (@Core.eval _ _ t Naive.translate)) x = Some y ->
+ stateShape x = stateShape y.
+Proof.
+unfold bump.
+repeat rewrite runMachine_seq.
+unfold fwd, runMachine at 3.
+destruct (Fwd_chk _) as [[[l0 st0] [_ ->]] |];[cbn|discriminate].
+set (x1 := fillReadFrame _ _); specialize (Ht x1).
+destruct (runMachine _ x1) as [y0|];[cbn|discriminate].
+specialize (Ht _ (refl_equal _)).
+unfold bwd, runMachine.
+destruct (Bwd_chk _) as [[[l1 st1] [_ ->]] |];[cbn|discriminate].
+intros Hxy.
+inversion_clear Hxy.
+unfold x1 in *; clear x1.
+repeat rewrite fillReadFrameShape_correct in *.
+cbn in *.
+do 2 rewrite rev_length, Nat.add_0_r in Ht.
+assumption.
+Qed.
+
+Lemma case_spec {A B C D : Ty} (s : Term (A * C) D) (t : Term (B * C) D) :
+ spec s -> spec t -> spec (case s t).
+Proof.
+intros Hs Ht x y; cbn.
+rewrite runMachine_choice.
+destruct (nextData _) as [| [[|] |] _]; try discriminate;
+apply bump_spec; auto.
+Qed.
+
+Lemma pair_spec {A B C : Ty} (s : Term A B) (t : Term A C) :
+ spec s -> spec t -> spec (pair s t).
+Proof.
+intros Hs Ht x z; cbn.
+rewrite runMachine_seq.
+specialize (Hs x).
+destruct (runMachine _ x) as [y|];[|discriminate].
+rewrite (Hs y);auto.
+Qed.
+
+Lemma take_spec {A B C : Ty} (t : Term A C) :
+ spec t -> spec (@take A B C t).
+Proof.
+auto.
+Qed.
+
+Lemma drop_spec {A B C : Ty} (t : Term B C) :
+ spec t -> spec (@drop A B C t).
+Proof.
+intros Ht x y; cbn.
+apply bump_spec.
+assumption.
+Qed.
+
+Lemma Core_spec {A B : Ty} (t : Term A B) :
+ spec t.
+Proof.
+induction t.
+- apply iden_spec.
+- apply comp_spec; assumption.
+- apply unit_spec.
+- apply injl_spec; assumption.
+- apply injr_spec; assumption.
+- apply case_spec; assumption.
+- apply pair_spec; assumption.
+- apply take_spec; assumption.
+- apply drop_spec; assumption.
+Qed.
+
+End StateShape.
+
+
+
+
+
+
